\documentclass{report}
\input{Preambolo}
\begin{document}
\section{3 nodi chiuso}
\begin{equation*}
\begin{aligned}
\dot{\angol {S_1}} = & -\tau \angol{ S_1 I_2}, \\
	\dot{\angol {I_1}} = & \spa \tau \angol{S_1 I_2}-\gamma \angol{I_1}, \\
	\dot{\angol {S_2}} = & -\tau \tonde{ \angol{ I_1 S_2} + \angol{S_2I_3}},	\\
	\dot{\angol {I_2}} = &\spa \tau \tonde{ \angol{ I_1 S_2} + \angol{S_2I_3}}-\gamma \angol{I_2}\\
	\dot{\angol {S_3}} = & -\tau \angol{ I_2 S_3},\\	\dot{\angol {I_3}} = & \spa \tau \angol{ I_2 S_3}-\gamma \angol{I_3},\\
 	\dot{\angol{S_1I_2}}=&\spa\tau\angol{S_1S_2I_3} - \tonde{ \tau + \gamma}\angol{S_1 I_2},
\\
	\dot{\angol{I_1S_2}}=&-\tau\angol{I_1S_2I_3} - \tonde{ \tau + \gamma}\angol{I_1 S_2},
\\
	\dot{\angol{S_2I_3}}=&-\tau\angol{I_1S_2I_3} - \tonde{ \tau + \gamma}\angol{S_2 I_3},
\\
	\dot{\angol{I_2S_3}}=&\spa\tau\angol{I_1S_2S_3} - \tonde{ \tau + \gamma}\angol{I_2 S_3}\\
	\dot{\angol{S_1S_2I_3}}=&-\tonde{\tau + \gamma}\angol{S_1S_2I_3},\\
	\dot{\angol{I_1S_2I_3}}=&-\tonde{2\tau + 2\gamma}\angol{I_1S_2I_3},\\
	\dot{\angol{I_1S_2S_3}}=&-\tonde{\tau + \gamma}\angol{I_1S_2S_3}.
\end{aligned}
\end{equation*}

\newpage
\section{3 nodi cut-vertex}
\begin{equation*}
\begin{aligned}
\dot{\angol {S_1}} = & -\tau \angol{ S_1 I_2}, \\
	\dot{\angol {I_1}} = & \spa \tau \angol{S_1 I_2}-\gamma \angol{I_1}, \\
	\dot{\angol {S_2}} = & -\tau \tonde{ \angol{ I_1 S_2} + \angol{S_2I_3}},	\\
	\dot{\angol {I_2}} = &\spa \tau \tonde{ \angol{ I_1 S_2} + \angol{S_2I_3}}-\gamma \angol{I_2}\\
	\dot{\angol {S_3}} = & -\tau \angol{ I_2 S_3},\\	\dot{\angol {I_3}} = & \spa \tau \angol{ I_2 S_3}-\gamma \angol{I_3},\\
 	\dot{\angol{S_1I_2}}=&\spa\tau\frac{\angol{S_1S_2}\angol{S_2I_3}}{\angol{S_2}} - \tonde{ \tau + \gamma}\angol{S_1 I_2},
\\
	\dot{\angol{I_1S_2}}=&-\tau\frac{\angol{I_1S_2}\angol{S_2I_3}}{\angol{S_2}} - \tonde{ \tau + \gamma}\angol{I_1 S_2},
\\
	\dot{\angol{S_2I_3}}=&-\tau\frac{\angol{I_1S_2}\angol{S_2I_3}}{\angol{S_2}} - \tonde{ \tau + \gamma}\angol{S_2 I_3},
\\
	\dot{\angol{I_2S_3}}=&\spa\tau\frac{\angol{I_1S_2}\angol{S_2S_3}}{\angol{S_2}} - \tonde{ \tau + \gamma}\angol{I_2 S_3}\\
	\dot{\angol{S_1S_2}} = &- \tau\frac{\angol{S_1S_2}\angol{S_2I_3}}{\angol{S_2}}\\
	\dot{\angol{S_2S_3}}= & -\tau \frac{\angol{ I_1 S_2}\angol{S_2S_3}}{\angol{S_3}}, 
\end{aligned}
\end{equation*}

\end{document}
